class SatisfiesProperties
move stuff to semantics_properties

minuska/theories/semantics_properties.v
@@ -5,6 +5,226 @@ From Minuska Require Import
     syntax_properties
 .
 
+Lemma Expression_evaluate_extensive_Some
+    {Σ : StaticModel}
+    (ρ1 ρ2 : gmap variable GroundTerm)
+    (t : Expression)
+    (gt : GroundTerm)
+    :
+    ρ1 ⊆ ρ2 ->
+    Expression_evaluate ρ1 t = Some gt ->
+    Expression_evaluate ρ2 t = Some gt.
+Proof.
+    intros Hρ1ρ2.
+    revert gt.
+    induction t; simpl; intros gt.
+    { ltac1:(tauto). }
+    {
+        unfold vars_of in Hρ1ρ2.
+        simpl in Hρ1ρ2.
+        intros H.
+        eapply (lookup_weaken ρ1 ρ2 x).
+        { apply H. }
+        { assumption. }
+    }
+    {
+        auto with nocore.
+    }
+    {
+        do 2 (rewrite bind_Some).
+        intros [x [Hx1 Hx2]].
+        exists x.
+        rewrite (IHt _ Hx1).
+        split>[reflexivity|].
+        assumption.
+    }
+    {
+        do 2 (rewrite bind_Some).
+        intros [x [Hx1 Hx2]].
+        exists x.
+        rewrite (IHt1 _ Hx1).
+        split>[reflexivity|].
+
+        rewrite bind_Some in Hx2.
+        destruct Hx2 as [x' [Hx'1 Hx'2]].
+        rewrite bind_Some.
+        exists x'.
+        rewrite (IHt2 _ Hx'1).
+        split>[reflexivity|].
+        assumption.
+    }
+    {
+        do 2 (rewrite bind_Some).
+        intros [x [Hx1 Hx2]].
+        exists x.
+        rewrite (IHt1 _ Hx1).
+        split>[reflexivity|].
+
+        rewrite bind_Some in Hx2.
+        destruct Hx2 as [x' [Hx'1 Hx'2]].
+        rewrite bind_Some.
+
+        rewrite bind_Some in Hx'2.
+        destruct Hx'2 as [x'' [Hx''1 Hx''2]].
+        exists x'.
+        rewrite (IHt2 _ Hx'1).
+        split>[reflexivity|].
+
+        rewrite bind_Some.
+        exists x''.
+        rewrite (IHt3 _ Hx''1).
+        split>[reflexivity|].
+        assumption.
+    }
+Qed.
+
+Lemma Expression_evaluate_extensive_None
+    {Σ : StaticModel}
+    (ρ1 ρ2 : gmap variable GroundTerm)
+    (t : Expression)
+    :
+    ρ1 ⊆ ρ2 ->
+    Expression_evaluate ρ2 t = None ->
+    Expression_evaluate ρ1 t = None.
+Proof.
+    intros Hρ1ρ2.
+    induction t; simpl.
+    { ltac1:(tauto). }
+    {
+        unfold vars_of in Hρ1ρ2.
+        simpl in Hρ1ρ2.
+        intros H.
+        eapply (lookup_weaken_None ρ1 ρ2 x).
+        { apply H. }
+        { assumption. }
+    }
+    {
+        auto with nocore.
+    }
+    {
+        do 2 (rewrite bind_None).
+        intros [HNone|Hrest].
+        {
+            specialize (IHt HNone).
+            rewrite IHt.
+            left. reflexivity.
+        }
+        destruct Hrest as [x [Hx1 Hx2]].
+        inversion Hx2.
+    }
+    {
+        do 2 (rewrite bind_None).
+        intros [HNone|Hrest].
+        {
+            specialize (IHt1 HNone).
+            rewrite IHt1.
+            left. reflexivity.
+        }
+        destruct Hrest as [x [Hx1 Hx2]].
+        rewrite bind_None in Hx2.
+        destruct Hx2 as [HNone|Hx2].
+        {
+            specialize (IHt2 HNone).
+            destruct (Expression_evaluate ρ1 t1).
+            {
+                right.
+                exists g.
+                split>[reflexivity|].
+                rewrite bind_None.
+                left. exact IHt2.
+            }
+            {
+                left. reflexivity.
+            }
+        }
+        {
+            destruct Hx2 as [x2 [Hx21 Hx22]].
+            inversion Hx22.
+        }
+    }
+    {
+        do 2 (rewrite bind_None).
+        intros [HNone|Hrest].
+        {
+            specialize (IHt1 HNone).
+            rewrite IHt1.
+            left. reflexivity.
+        }
+        destruct Hrest as [x [Hx1 Hx2]].
+        rewrite bind_None in Hx2.
+        destruct Hx2 as [HNone|Hx2].
+        {
+            specialize (IHt2 HNone).
+            destruct (Expression_evaluate ρ1 t1).
+            {
+                right.
+                exists g.
+                split>[reflexivity|].
+                rewrite bind_None.
+                left. exact IHt2.
+            }
+            {
+                left. reflexivity.
+            }
+        }
+        destruct Hx2 as [x' [Hx'1 Hx'2]].
+        rewrite bind_None in Hx'2.
+        destruct Hx'2 as [HNone|Hx'2].
+        {
+            specialize (IHt3 HNone).
+            destruct (Expression_evaluate ρ1 t1).
+            {
+                right.
+                exists g.
+                split>[reflexivity|].
+                rewrite bind_None.
+
+                destruct (Expression_evaluate ρ1 t2).
+                {
+                    right.
+                    exists g0.
+                    split>[reflexivity|].
+                    rewrite bind_None.
+                    left. exact IHt3.
+                }
+                {
+                    left. reflexivity.
+                }
+            }
+            {
+                left. reflexivity.
+            }
+        }
+        {
+            destruct Hx'2 as [x2 [Hx'21 Hx'22]].
+            inversion Hx'22.
+        }
+    }
+Qed.
+
+
+Lemma Expression_evaluate_extensive'
+    {Σ : StaticModel}
+    (ρ1 ρ2 : gmap variable GroundTerm)
+    (t : Expression)
+    :
+    ρ1 ⊆ ρ2 ->
+    isSome (Expression_evaluate ρ1 t) ->
+    Expression_evaluate ρ1 t = Expression_evaluate ρ2 t.
+Proof.
+    intros H1 H2.
+    unfold isSome in H2.
+    ltac1:(case_match).
+    {
+        symmetry.
+        eapply Expression_evaluate_extensive_Some in H>[|apply H1].
+        assumption.
+    }
+    {
+        inversion H2.
+    }
+Qed.
+
 Lemma Expression_evalute_total_iff
     {Σ : StaticModel}
     (t : Expression)
@@ -120,25 +340,539 @@ Proof.
     }
 Qed.
 
-(*
-Lemma Expression_evaluate_eq
+Class SatisfiesProperties
     {Σ : StaticModel}
-    (ρ1 ρ2 : gmap variable GroundTerm)
-    (t : Expression)
-    :
-    vars_of t ⊆ vars_of ρ1 ->
-    vars_of t ⊆ vars_of ρ2 ->
-    Expression_evaluate ρ1 t = Expression_evaluate ρ2 t.
-Proof.
-    intros H1 H2.
-    induction t; simpl.
-    { reflexivity. }
-    {
-        unfold vars_of in *; simpl in *.
-    }
+    (V A B var : Type)
+    {_SV : SubsetEq V}
+    {_varED : EqDecision var}
+    {_varCnt : Countable var}
+    {_VV: VarsOf V var}
+    {_SAT : Satisfies V A B var}
+    :=
+mkSatisfiesProperties {
+    satisfies_ext :
+        forall (v1 v2 : V),
+            v1 ⊆ v2 ->
+            forall (a : A) (b : B),
+                satisfies v1 a b ->
+                satisfies v2 a b ;
+}.
 
+#[export]
+Instance SatisfiesProperties_val_ap
+    {Σ : StaticModel} :
+    SatisfiesProperties
+        (gmap variable GroundTerm)
+        unit
+        AtomicProposition
+        variable
+.
+Proof.
+    constructor. intros.
+    destruct b; simpl in *.
+    {
+        destruct H0 as [H1 [x Hx]].
+        unfold satisfies; simpl.
+        rewrite (Expression_evaluate_extensive_Some v1 v2 _ x H Hx).
+        split>[|eexists; reflexivity].
+        rewrite H1 in Hx.
+        rewrite (Expression_evaluate_extensive_Some v1 v2 e2 x H Hx).
+        reflexivity.
+    }
 Qed.
-*)
+
+
+#[export]
+Instance SatisfiesProperties_builtin_BuiltinOrVar
+    {Σ : StaticModel}
+    :
+    SatisfiesProperties Valuation (builtin_value) BuiltinOrVar variable
+.
+Proof.
+    constructor. intros.
+    inversion H0; constructor.
+    {
+        subst.
+        unfold Valuation in *.
+        eapply lookup_weaken.
+        { apply H1. }
+        { assumption. }
+    }
+Qed.
+
+
+#[export]
+Instance SatisfiesProperties__AppliedOperator'_symbol_builtin__BuiltinOrVar
+    {Σ : StaticModel}
+    : SatisfiesProperties Valuation ((AppliedOperator' symbol builtin_value)) BuiltinOrVar variable
+.
+Proof.
+    constructor. intros.
+    destruct b; simpl in *.
+    { ltac1:(contradiction). }
+    {
+        unfold satisfies; simpl.
+        unfold Valuation in *.
+        eapply lookup_weaken.
+        { apply H0. }
+        { assumption. }
+    }
+Qed.
+
+Instance SatisfiesProperties_AppliedOperator'_symbol_builtin_BuiltinOrVar
+    {Σ : StaticModel}
+    :
+    SatisfiesProperties Valuation ((AppliedOperator' symbol builtin_value)) BuiltinOrVar variable
+.
+Proof.
+    constructor. intros.
+    destruct b; simpl in *.
+    { ltac1:(contradiction). }
+    {
+        unfold satisfies; simpl.
+        unfold Valuation in *.
+        eapply lookup_weaken.
+        { apply H0. }
+        { assumption. }
+    }
+Qed.
+
+
+#[export]
+Instance SatisfiesProperties__builtin__ao'B
+    {Σ : StaticModel}
+    {V B var : Type}
+    {_SV : SubsetEq V}
+    {_EDv : EqDecision var}
+    {_Cv : Countable var}
+    {_VV : VarsOf V var}
+    :
+    SatisfiesProperties
+        V
+        (builtin_value)
+        (AppliedOperator' symbol B)
+        var
+.
+Proof.
+    constructor. intros. auto.
+Qed.
+
+
+#[export]
+Instance SatisfiesProperties_aoxyo_aoxzo
+    {Σ : StaticModel}
+    (V X Y Z var : Type)
+    {_varED : EqDecision var}
+    {_varCnt : Countable var}
+    {_VV : VarsOf V var}
+    {_SV : SubsetEq V}
+    {_S1 : Satisfies V Y Z var}
+    {_S2 : Satisfies V ((AppliedOperator' X Y)) Z var}
+    {_S3 : Satisfies V ((AppliedOperator' X Y)) (AppliedOperator' X Z) var}
+    {_S1P : SatisfiesProperties V Y Z var}
+    {_S2P : SatisfiesProperties V ((AppliedOperator' X Y)) Z var}
+    {_S3P : SatisfiesProperties V ((AppliedOperator' X Y)) (AppliedOperator' X Z) var}
+    :
+    SatisfiesProperties V ((AppliedOperatorOr' X Y)) (AppliedOperatorOr' X Z) var
+.
+Proof.
+    constructor. intros.
+    destruct H0; constructor.
+    {
+        eapply satisfies_ext.
+        { exact H. }
+        { exact pf. }
+    }
+    {
+        eapply satisfies_ext.
+        { exact H. }
+        { exact pf. }
+    }
+    {
+        eapply satisfies_ext.
+        { exact H. }
+        { assumption. }
+    }
+Qed.
+
+
+
+Instance SatisfiesProperties_aoxy_aoxz
+    {Σ : StaticModel}
+    {V X Y Z var : Type}
+    {_varED : EqDecision var}
+    {_varCnt : Countable var}
+    {_VV : VarsOf V var}
+    {_SV : SubsetEq V}
+    {_S1 : Satisfies V (Y) Z var}
+    {_S2 : Satisfies V (Y) (AppliedOperator' X Z) var}
+    {_S3 : Satisfies V ((AppliedOperator' X Y)) Z var}
+    {_S1P : SatisfiesProperties V (Y) Z var}
+    {_S2P : SatisfiesProperties V (Y) (AppliedOperator' X Z) var}
+    {_S3P : SatisfiesProperties V ((AppliedOperator' X Y)) Z var}
+    :
+    SatisfiesProperties V ((AppliedOperator' X Y)) (AppliedOperator' X Z) var
+.
+Proof.
+    constructor. intros.
+    revert v2 H.
+    induction H0; intros v2 HH; constructor; try (ltac1:(naive_solver)).
+    {
+        eapply satisfies_ext.
+        { apply HH. }
+        { exact H. }
+    }
+    {
+        eapply satisfies_ext.
+        { apply HH. }
+        { exact H. }
+    }
+    {
+        eapply satisfies_ext.
+        { apply HH. }
+        { exact H. }
+    }
+Qed.
+
+#[export]
+Instance SatisfiesProperties_aoosb_aoosbf
+    {Σ : StaticModel}
+    :
+    SatisfiesProperties
+        Valuation
+        ((AppliedOperatorOr' symbol builtin_value))
+        (AppliedOperatorOr' symbol BuiltinOrVar)
+        variable
+.
+Proof.
+    apply SatisfiesProperties_aoxyo_aoxzo.
+    {
+        apply _.
+    }
+    {
+        apply _.
+    }
+    {
+        apply _.
+    }
+Defined.
+
+#[export]
+Instance SatisfiesProperties_valGroundTerm_OpenTerm
+    {Σ : StaticModel}
+    :
+    SatisfiesProperties
+        Valuation
+        GroundTerm
+        OpenTerm
+        variable
+.
+Proof.
+    apply _.
+Defined.
+
+#[export]
+Instance SatisfiesProperties_val_match
+    {Σ : StaticModel}
+    :
+    SatisfiesProperties
+        Valuation
+        unit
+        Match
+        variable
+.
+Proof.
+    constructor. intros. unfold satisfies in *; simpl.
+    destruct b. simpl in *.
+    unfold Valuation in *.
+    ltac1:(repeat case_match).
+    {
+        eapply lookup_weaken in H1>[|apply H].
+        ltac1:(simplify_eq/=).
+        eapply satisfies_ext.
+        { apply H. }
+        { assumption. }
+    }
+    {
+        eapply lookup_weaken in H1>[|apply H].
+        ltac1:(simplify_eq/=).
+    }
+    {
+        ltac1:(contradiction).
+    }
+    {
+        ltac1:(contradiction).
+    }
+Qed.
+
+
+#[export]
+Instance SatisfiesProperties_val_sc
+    {Σ : StaticModel}
+    :
+    SatisfiesProperties
+        Valuation
+        unit
+        SideCondition
+        variable
+.
+Proof.
+    constructor. intros; unfold satisfies in *; simpl in *.
+    destruct b; simpl in *; eapply satisfies_ext>[apply H|]; assumption.
+Qed.
+
+Instance SatisfiesProperties_GroundTerm_BuiltinOrVar
+    {Σ : StaticModel}
+    :
+    SatisfiesProperties Valuation (GroundTerm) BuiltinOrVar variable
+.
+Proof.
+    constructor. unfold satisfies; simpl. intros.
+    destruct a,b; simpl in *; try ltac1:(naive_solver);
+        unfold Valuation in *; eapply lookup_weaken>[|apply H];
+        assumption.
+Qed.
+
+#[export]
+Instance SatisfiesProperties_builtin_value_OpenTerm
+    {Σ : StaticModel}
+    :
+    SatisfiesProperties
+        Valuation
+        builtin_value
+        OpenTerm
+        variable
+.
+Proof.
+    constructor. unfold satisfies; simpl. intros.
+    destruct b; simpl in *.
+    { assumption. }
+    {
+        eapply satisfies_ext>[apply H|].
+        assumption.
+    }
+Qed.
+
+
+#[export]
+Instance SatisfiesProperties__AppliedOperator'_symbol_builtin_value__BOV
+    {Σ : StaticModel}
+    {V : Type}
+    :
+    SatisfiesProperties
+        Valuation
+        ((AppliedOperator' symbol builtin_value))
+        BuiltinOrVar
+        variable
+.
+Proof.
+    constructor. unfold satisfies; simpl. intros.
+    destruct b; simpl in *; try assumption.
+    {
+        unfold Valuation in *.
+        eapply lookup_weaken.
+        { apply H0. }
+        { assumption. }
+    }
+Qed.
+
+#[export]
+Instance SatisfiesProperties__lift_builtin_to_aosb
+    {Σ : StaticModel}
+    {V A B var : Type}
+    {_varED : EqDecision var}
+    {_varCnt : Countable var}
+    {_SV : SubsetEq V}
+    {_VV : VarsOf V var}
+    {_S1 : Satisfies V (A) B var}
+    {_S2 : Satisfies V ((AppliedOperator' symbol A)) B var}
+    {_S3 : Satisfies V (AppliedOperator' symbol A) (AppliedOperator' symbol B) var}
+    {_S1P : SatisfiesProperties V (A) B var}
+    {_S2P : SatisfiesProperties V ((AppliedOperator' symbol A)) B var}
+    {_S3P : SatisfiesProperties V (AppliedOperator' symbol A) (AppliedOperator' symbol B) var}
+    :
+    SatisfiesProperties
+        V
+        ((AppliedOperator' symbol A))
+        (AppliedOperatorOr' symbol B)
+        var
+.
+Proof.
+    constructor. unfold satisfies; simpl. intros.
+    unfold AppliedOperator'_symbol_A_satisfies_OpenTermB' in *.
+    eapply satisfies_ext.
+    { apply H. }
+    { assumption. }
+Qed.    
+
+#[export]
+Instance SatisfiesProperties__AppliedOperator'_symbol_builtin__OpenTerm
+    {Σ : StaticModel}
+    {V var : Type}
+    {_varED : EqDecision var}
+    {_varCnt : Countable var}
+    {_SV : SubsetEq V}
+    {_VV : VarsOf V var}
+    {_S1 : Satisfies V (builtin_value) BuiltinOrVar var}
+    {_S2 : Satisfies V (AppliedOperator' symbol builtin_value) BuiltinOrVar var}
+    {_S3 : Satisfies V (AppliedOperator' symbol builtin_value) (AppliedOperator' symbol BuiltinOrVar) var}
+    {_S1P : SatisfiesProperties V (builtin_value) BuiltinOrVar var}
+    {_S2P : SatisfiesProperties V (AppliedOperator' symbol builtin_value) BuiltinOrVar var}
+    {_S3P : SatisfiesProperties V (AppliedOperator' symbol builtin_value) (AppliedOperator' symbol BuiltinOrVar) var}
+    :
+    SatisfiesProperties V
+        ((AppliedOperator' symbol builtin_value))
+        OpenTerm
+        var
+.
+Proof.
+    constructor. unfold satisfies. simpl. intros.
+    eapply satisfies_ext.
+    { apply H. }
+    { assumption. }
+Qed.
+
+Instance SatisfiesProperties_builtin_expr
+    {Σ : StaticModel}:
+    SatisfiesProperties
+        Valuation
+        builtin_value
+        Expression
+        variable
+.
+Proof.
+    constructor. unfold satisfies. simpl.  intros. simpl in *.
+    erewrite Expression_evaluate_extensive_Some>[|apply H|].
+    { reflexivity. }
+    { assumption. }
+Qed.
+
+
+#[export]
+Instance SatisfiesProperties_asb_expr
+    {Σ : StaticModel}:
+    SatisfiesProperties
+        Valuation
+        ((AppliedOperator' symbol builtin_value))
+        Expression
+        variable
+.
+Proof.
+    constructor. unfold satisfies. simpl. intros. simpl in *.
+    erewrite Expression_evaluate_extensive_Some>[|apply H|].
+    { reflexivity. }
+    { assumption. }
+Qed.
+
+#[export]
+Instance SatisfiesProperties_gt_var
+    {Σ : StaticModel}:
+    SatisfiesProperties
+        Valuation
+        GroundTerm
+        variable
+        variable
+.
+Proof.
+    constructor. unfold satisfies. simpl. intros. simpl in *.
+    unfold Valuation in *.
+    eapply lookup_weaken.
+    { apply H0. }
+    { assumption. }
+Qed.
+
+
+#[export]
+Instance SatisfiesProperties_sym_bov
+    {Σ : StaticModel}
+    :
+    SatisfiesProperties
+        Valuation
+        symbol
+        BuiltinOrVar
+        variable
+.
+Proof.
+    constructor. unfold satisfies. simpl. 
+    simpl. auto with nocore.
+Qed.
+
+#[export]
+Instance SatisfiesProperties_Valuation_LR_SideCondition
+    {Σ : StaticModel}
+    :
+    SatisfiesProperties
+        (Valuation * LeftRight)
+        unit
+        SideCondition
+        variable
+.
+Proof.
+    constructor. unfold satisfies. simpl. 
+    simpl. intros.
+    inversion H; subst.
+    eapply satisfies_ext.
+    { apply H1. }
+    { assumption. }
+Qed.
+
+
+#[export]
+Instance SatisfiesProperties__GroundTerm__OpenTerm_inall
+    {Σ : StaticModel}
+    :
+    SatisfiesProperties
+        unit
+        GroundTerm
+        OpenTerm
+        variable
+.
+Proof.
+    constructor. unfold satisfies. simpl. 
+    simpl. intros. assumption.
+Qed.
+
+
+#[export]
+Instance SatisfiesProperties_valuation_scs
+    {Σ : StaticModel}
+    : SatisfiesProperties
+        Valuation
+        unit
+        (list SideCondition)
+        variable
+.
+Proof.
+    constructor. unfold satisfies. simpl. 
+    intros. simpl in *.
+    rewrite Forall_forall. rewrite Forall_forall in H0.
+    intros x Hx. specialize (H0 x Hx).
+    eapply satisfies_ext.
+    { apply H. }
+    { assumption. }
+Qed.
+
+
+#[export]
+Instance
+    SatisfiesProperties_symbol_B
+    {Σ : StaticModel}
+    {V B var : Type}
+    {_SV : SubsetEq V}
+    {_EDvar : EqDecision var}
+    {_Covar : Countable var}
+    {_VV : VarsOf V var}
+    :
+    SatisfiesProperties
+        V
+        symbol
+        B
+        var
+.
+Proof.
+    constructor. unfold satisfies. simpl.     
+    auto with nocore.
+Qed.
 
 Lemma Expression_evalute_total_same
     {Σ : StaticModel}
