minuska/theories/spec_semantics.v
@@ -64,225 +64,6 @@ match t with
 end.
 
 
-Lemma Expression_evaluate_extensive_Some
-    {Σ : StaticModel}
-    (ρ1 ρ2 : gmap variable GroundTerm)
-    (t : Expression)
-    (gt : GroundTerm)
-    :
-    ρ1 ⊆ ρ2 ->
-    Expression_evaluate ρ1 t = Some gt ->
-    Expression_evaluate ρ2 t = Some gt.
-Proof.
-    intros Hρ1ρ2.
-    revert gt.
-    induction t; simpl; intros gt.
-    { ltac1:(tauto). }
-    {
-        unfold vars_of in Hρ1ρ2.
-        simpl in Hρ1ρ2.
-        intros H.
-        eapply (lookup_weaken ρ1 ρ2 x).
-        { apply H. }
-        { assumption. }
-    }
-    {
-        auto with nocore.
-    }
-    {
-        do 2 (rewrite bind_Some).
-        intros [x [Hx1 Hx2]].
-        exists x.
-        rewrite (IHt _ Hx1).
-        split>[reflexivity|].
-        assumption.
-    }
-    {
-        do 2 (rewrite bind_Some).
-        intros [x [Hx1 Hx2]].
-        exists x.
-        rewrite (IHt1 _ Hx1).
-        split>[reflexivity|].
-
-        rewrite bind_Some in Hx2.
-        destruct Hx2 as [x' [Hx'1 Hx'2]].
-        rewrite bind_Some.
-        exists x'.
-        rewrite (IHt2 _ Hx'1).
-        split>[reflexivity|].
-        assumption.
-    }
-    {
-        do 2 (rewrite bind_Some).
-        intros [x [Hx1 Hx2]].
-        exists x.
-        rewrite (IHt1 _ Hx1).
-        split>[reflexivity|].
-
-        rewrite bind_Some in Hx2.
-        destruct Hx2 as [x' [Hx'1 Hx'2]].
-        rewrite bind_Some.
-
-        rewrite bind_Some in Hx'2.
-        destruct Hx'2 as [x'' [Hx''1 Hx''2]].
-        exists x'.
-        rewrite (IHt2 _ Hx'1).
-        split>[reflexivity|].
-
-        rewrite bind_Some.
-        exists x''.
-        rewrite (IHt3 _ Hx''1).
-        split>[reflexivity|].
-        assumption.
-    }
-Qed.
-
-Lemma Expression_evaluate_extensive_None
-    {Σ : StaticModel}
-    (ρ1 ρ2 : gmap variable GroundTerm)
-    (t : Expression)
-    :
-    ρ1 ⊆ ρ2 ->
-    Expression_evaluate ρ2 t = None ->
-    Expression_evaluate ρ1 t = None.
-Proof.
-    intros Hρ1ρ2.
-    induction t; simpl.
-    { ltac1:(tauto). }
-    {
-        unfold vars_of in Hρ1ρ2.
-        simpl in Hρ1ρ2.
-        intros H.
-        eapply (lookup_weaken_None ρ1 ρ2 x).
-        { apply H. }
-        { assumption. }
-    }
-    {
-        auto with nocore.
-    }
-    {
-        do 2 (rewrite bind_None).
-        intros [HNone|Hrest].
-        {
-            specialize (IHt HNone).
-            rewrite IHt.
-            left. reflexivity.
-        }
-        destruct Hrest as [x [Hx1 Hx2]].
-        inversion Hx2.
-    }
-    {
-        do 2 (rewrite bind_None).
-        intros [HNone|Hrest].
-        {
-            specialize (IHt1 HNone).
-            rewrite IHt1.
-            left. reflexivity.
-        }
-        destruct Hrest as [x [Hx1 Hx2]].
-        rewrite bind_None in Hx2.
-        destruct Hx2 as [HNone|Hx2].
-        {
-            specialize (IHt2 HNone).
-            destruct (Expression_evaluate ρ1 t1).
-            {
-                right.
-                exists g.
-                split>[reflexivity|].
-                rewrite bind_None.
-                left. exact IHt2.
-            }
-            {
-                left. reflexivity.
-            }
-        }
-        {
-            destruct Hx2 as [x2 [Hx21 Hx22]].
-            inversion Hx22.
-        }
-    }
-    {
-        do 2 (rewrite bind_None).
-        intros [HNone|Hrest].
-        {
-            specialize (IHt1 HNone).
-            rewrite IHt1.
-            left. reflexivity.
-        }
-        destruct Hrest as [x [Hx1 Hx2]].
-        rewrite bind_None in Hx2.
-        destruct Hx2 as [HNone|Hx2].
-        {
-            specialize (IHt2 HNone).
-            destruct (Expression_evaluate ρ1 t1).
-            {
-                right.
-                exists g.
-                split>[reflexivity|].
-                rewrite bind_None.
-                left. exact IHt2.
-            }
-            {
-                left. reflexivity.
-            }
-        }
-        destruct Hx2 as [x' [Hx'1 Hx'2]].
-        rewrite bind_None in Hx'2.
-        destruct Hx'2 as [HNone|Hx'2].
-        {
-            specialize (IHt3 HNone).
-            destruct (Expression_evaluate ρ1 t1).
-            {
-                right.
-                exists g.
-                split>[reflexivity|].
-                rewrite bind_None.
-
-                destruct (Expression_evaluate ρ1 t2).
-                {
-                    right.
-                    exists g0.
-                    split>[reflexivity|].
-                    rewrite bind_None.
-                    left. exact IHt3.
-                }
-                {
-                    left. reflexivity.
-                }
-            }
-            {
-                left. reflexivity.
-            }
-        }
-        {
-            destruct Hx'2 as [x2 [Hx'21 Hx'22]].
-            inversion Hx'22.
-        }
-    }
-Qed.
-
-
-Lemma Expression_evaluate_extensive'
-    {Σ : StaticModel}
-    (ρ1 ρ2 : gmap variable GroundTerm)
-    (t : Expression)
-    :
-    ρ1 ⊆ ρ2 ->
-    isSome (Expression_evaluate ρ1 t) ->
-    Expression_evaluate ρ1 t = Expression_evaluate ρ2 t.
-Proof.
-    intros H1 H2.
-    unfold isSome in H2.
-    ltac1:(case_match).
-    {
-        symmetry.
-        eapply Expression_evaluate_extensive_Some in H>[|apply H1].
-        assumption.
-    }
-    {
-        inversion H2.
-    }
-Qed.
 
 Class Satisfies
     {Σ : StaticModel}
@@ -295,16 +76,10 @@ Class Satisfies
 mkSatisfies {
     satisfies :
         V -> A -> B -> Prop ;
-
-    satisfies_ext :
-        forall (v1 v2 : V),
-            v1 ⊆ v2 ->
-            forall (a : A) (b : B),
-                satisfies v1 a b ->
-                satisfies v2 a b ;
 }.
 
 Arguments satisfies : simpl never.
+
 
 Definition val_satisfies_ap
     {Σ : StaticModel} (ρ : Valuation) (ap : AtomicProposition)
@@ -328,19 +103,7 @@ Program Instance Satisfies_val_ap
 := {|
     satisfies := fun ρ u ap => val_satisfies_ap ρ ap ;
 |}.
-Next Obligation.
-    destruct b; simpl in *.
-    {
-        intros H0.
-        destruct H0 as [H1 [x Hx]].
-        rewrite (Expression_evaluate_extensive_Some v1 v2 _ x H Hx).
-        split>[|eexists; reflexivity].
-        rewrite H1 in Hx.
-        rewrite (Expression_evaluate_extensive_Some v1 v2 e2 x H Hx).
-        reflexivity.
-    }
-Qed.
-Fail Next Obligation.
+
 
 Inductive aoxy_satisfies_aoxz
     {Σ : StaticModel}
@@ -410,7 +173,7 @@ Inductive aoxy_satisfies_aoxz
 
 
 #[export]
-Program Instance Satisfies_aoxy_aoxz
+Instance Satisfies_aoxy_aoxz
     {Σ : StaticModel}
     {V X Y Z var : Type}
     {_varED : EqDecision var}
@@ -425,27 +188,6 @@ Program Instance Satisfies_aoxy_aoxz
 := {|
     satisfies := aoxy_satisfies_aoxz ;
 |}.
-Next Obligation.
-    intros.
-    revert v2 H.
-    induction H0; intros v2 HH; constructor; try (ltac1:(naive_solver)).
-    {
-        eapply satisfies_ext.
-        { apply HH. }
-        { exact H. }
-    }
-    {
-        eapply satisfies_ext.
-        { apply HH. }
-        { exact H. }
-    }
-    {
-        eapply satisfies_ext.
-        { apply HH. }
-        { exact H. }
-    }
-Qed.
-Fail Next Obligation.
 
 
 Inductive aoxyo_satisfies_aoxzo
@@ -497,26 +239,6 @@ Program Instance Satisfies_aoxyo_aoxzo
 := {|
     satisfies := aoxyo_satisfies_aoxzo V X Y Z var;
 |}.
-Next Obligation.
-    intros.
-    destruct H0; constructor.
-    {
-        eapply satisfies_ext.
-        { exact H. }
-        { exact pf. }
-    }
-    {
-        eapply satisfies_ext.
-        { exact H. }
-        { exact pf. }
-    }
-    {
-        eapply satisfies_ext.
-        { exact H. }
-        { assumption. }
-    }
-Qed.
-Fail Next Obligation.
 
 Inductive builtin_satisfies_BuiltinOrVar
     {Σ : StaticModel}
@@ -554,25 +276,13 @@ Proof.
 Defined.
 
 #[export]
-Program Instance Satisfies_builtin_BuiltinOrVar
+Instance Satisfies_builtin_BuiltinOrVar
     {Σ : StaticModel}
     :
     Satisfies Valuation (builtin_value) BuiltinOrVar variable
 := {|
     satisfies := builtin_satisfies_BuiltinOrVar' ;
 |}.
-Next Obligation.
-    intros.
-    inversion H0; constructor.
-    {
-        subst.
-        unfold Valuation in *.
-        eapply lookup_weaken.
-        { apply H1. }
-        { assumption. }
-    }
-Qed.
-Fail Next Obligation.
 
 Definition AppliedOperator'_symbol_builtin_satisfies_BuiltinOrVar
     {Σ : StaticModel}
@@ -592,18 +302,6 @@ Program Instance Satisfies__AppliedOperator'_symbol_builtin__BuiltinOrVar
 := {| 
     satisfies := AppliedOperator'_symbol_builtin_satisfies_BuiltinOrVar
 |}.
-Next Obligation.
-    intros.
-    destruct b; simpl in *.
-    { ltac1:(contradiction). }
-    {
-        unfold Valuation in *.
-        eapply lookup_weaken.
-        { apply H0. }
-        { assumption. }
-    }
-Qed.
-Fail Next Obligation.
 
 Definition AppliedOperator'_symbol_builtin_satisfies'_BuiltinOrVar
     {Σ : StaticModel}
@@ -614,25 +312,13 @@ Definition AppliedOperator'_symbol_builtin_satisfies'_BuiltinOrVar
 := AppliedOperator'_symbol_builtin_satisfies_BuiltinOrVar ρ aop bov.
 
 #[export]
-Program Instance Satisfies_AppliedOperator'_symbol_builtin_BuiltinOrVar
+Instance Satisfies_AppliedOperator'_symbol_builtin_BuiltinOrVar
     {Σ : StaticModel}
     :
     Satisfies Valuation ((AppliedOperator' symbol builtin_value)) BuiltinOrVar variable
 := {|
     satisfies := AppliedOperator'_symbol_builtin_satisfies'_BuiltinOrVar ;
 |}.
-Next Obligation.
-    intros.
-    destruct b; simpl in *.
-    { ltac1:(contradiction). }
-    {
-        unfold Valuation in *.
-        eapply lookup_weaken.
-        { apply H0. }
-        { assumption. }
-    }
-Qed.
-Fail Next Obligation.
 
 (*
 Definition aosb_satisfies_aosbf
@@ -661,7 +347,7 @@ Definition aosb_satisfies_aosbf
 *)
 
 #[export]
-Program Instance Satisfies__builtin__ao'B
+Instance Satisfies__builtin__ao'B
     {Σ : StaticModel}
     {V B var : Type}
     {_SV : SubsetEq V}
@@ -677,10 +363,7 @@ Program Instance Satisfies__builtin__ao'B
 := {| 
     satisfies := fun _ _ _ => false ;
 |}.
-Next Obligation.
-    intros. auto.
-Qed.
-Fail Next Obligation.
+
 
 #[export]
 Instance Satisfies_aos__builtin_BuiltinOrVar
@@ -720,22 +403,6 @@ Proof.
     apply _.
 Defined.
 
-(*
-Definition aoosb_satisfies_aoosbf
-    {Σ : StaticModel}
-    :
-    Valuation ->
-    (AppliedOperatorOr' symbol builtin_value) ->
-    AppliedOperatorOr' symbol BuiltinOrVar ->
-    Prop :=
-    aoxyo_satisfies_aoxzo
-        Valuation
-        symbol
-        builtin_value
-        BuiltinOrVar
-.
-*)
-
 #[export]
 Instance
 Satisfies_aoosb_aoosbf
@@ -749,16 +416,6 @@ Satisfies_aoosb_aoosbf
 .
 Proof. apply _. Defined.
 
-(*
-Definition in_val_GroundTerm_satisfies_OpenTerm
-    {Σ : StaticModel}
-    (ρ : Valuation)
-    (g : GroundTerm)
-    (φ : OpenTerm)
-    : Prop := aoosb_satisfies_aoosbf ρ g φ
-.
-*)
-
 #[export]
 Instance Satisfies_valGroundTerm_OpenTerm
     {Σ : StaticModel}
@@ -769,7 +426,10 @@ Instance Satisfies_valGroundTerm_OpenTerm
         OpenTerm
         variable
 .
-Proof. apply _. Defined.
+Proof. 
+    apply _.
+Defined.
+Print Satisfies_valGroundTerm_OpenTerm.
 
 Definition valuation_satisfies_match
     {Σ : StaticModel}
@@ -796,30 +456,7 @@ Program Instance Satisfies_val_match
 := {|
     satisfies := fun a b c => valuation_satisfies_match a c;
 |}.
-Next Obligation.
-    intros.
-    destruct b. simpl in *.
-    unfold Valuation in *.
-    ltac1:(repeat case_match).
-    {
-        eapply lookup_weaken in H1>[|apply H].
-        ltac1:(simplify_eq/=).
-        eapply satisfies_ext.
-        { apply H. }
-        { assumption. }
-    }
-    {
-        eapply lookup_weaken in H1>[|apply H].
-        ltac1:(simplify_eq/=).
-    }
-    {
-        ltac1:(contradiction).
-    }
-    {
-        ltac1:(contradiction).
-    }
-Qed.
-Fail Next Obligation.
+
 
 Definition valuation_satisfies_sc
     {Σ : StaticModel}
@@ -831,7 +468,7 @@ match sc with
 end.
 
 #[export]
-Program Instance Satisfies_val_sc
+Instance Satisfies_val_sc
     {Σ : StaticModel}
     :
     Satisfies
@@ -842,11 +479,6 @@ Program Instance Satisfies_val_sc
 := {|
     satisfies := fun a b c => valuation_satisfies_sc a c ;
 |}.
-Next Obligation.
-    intros.
-    destruct b; simpl in *; eapply satisfies_ext>[apply H|]; assumption.
-Qed.
-Fail Next Obligation.
 
 
 Definition GroundTerm_satisfies_BuiltinOrVar
@@ -865,35 +497,13 @@ match bov with
 end.
 
 #[export]
-Program Instance Satisfies_GroundTerm_BuiltinOrVar
+Instance Satisfies_GroundTerm_BuiltinOrVar
     {Σ : StaticModel}
     :
     Satisfies Valuation (GroundTerm) BuiltinOrVar variable
 := {|
     satisfies := GroundTerm_satisfies_BuiltinOrVar ;
 |}.
-Next Obligation.
-    intros.
-    destruct a,b; simpl in *; try ltac1:(naive_solver);
-        unfold Valuation in *; eapply lookup_weaken>[|apply H];
-        assumption.
-Qed.
-Fail Next Obligation.
-
-(*
-Definition in_val_GroundTerm_satisfies_OpenTermWSC
-    {Σ : StaticModel}
-    :
-    Valuation ->
-    GroundTerm ->
-    OpenTermWSC ->
-    Prop :=
-    A_satisfies_B_WithASideCondition
-        Valuation
-        GroundTerm
-        OpenTerm
-.
-*)
 
 
 Definition builtin_value_satisfies_OpenTerm
@@ -910,7 +520,7 @@ match t with
 end.
 
 #[export]
-Program Instance Satisfies_builtin_value_OpenTerm
+Instance Satisfies_builtin_value_OpenTerm
     {Σ : StaticModel}
     :
     Satisfies
@@ -921,31 +531,6 @@ Program Instance Satisfies_builtin_value_OpenTerm
 := {|
     satisfies :=  builtin_value_satisfies_OpenTerm ;
 |}.
-Next Obligation.
-    intros.
-    destruct b; simpl in *.
-    { assumption. }
-    {
-        eapply satisfies_ext>[apply H|].
-        assumption.
-    }
-Qed.
-Fail Next Obligation.
-
-(*
-Definition builtin_value_satisfies_OpenTermWSC
-    {Σ : StaticModel}
-    :
-    Valuation ->
-    builtin_value ->
-    OpenTermWSC ->
-    Prop :=
-    A_satisfies_B_WithASideCondition
-        Valuation
-        builtin_value
-        OpenTerm
-.
-*)
 
 Definition AppliedOperator'_symbol_builtin_value_satisfies_BOV
     {Σ : StaticModel}
@@ -961,7 +546,7 @@ end
 .
 
 #[export]
-Program Instance Satisfies__AppliedOperator'_symbol_builtin_value__BOV
+Instance Satisfies__AppliedOperator'_symbol_builtin_value__BOV
     {Σ : StaticModel}
     {V : Type}
     :
@@ -973,17 +558,6 @@ Program Instance Satisfies__AppliedOperator'_symbol_builtin_value__BOV
 := {|
     satisfies := AppliedOperator'_symbol_builtin_value_satisfies_BOV;
 |}.
-Next Obligation.
-    intros.
-    destruct b; simpl in *; try assumption.
-    {
-        unfold Valuation in *.
-        eapply lookup_weaken.
-        { apply H0. }
-        { assumption. }
-    }
-Qed.
-Fail Next Obligation.
 
 Definition AppliedOperator'_symbol_A_satisfies_OpenTermB'
     {Σ : StaticModel}
@@ -1006,7 +580,7 @@ Definition AppliedOperator'_symbol_A_satisfies_OpenTermB'
 .
 
 #[export]
-Program Instance Satisfies__lift_builtin_to_aosb
+Instance Satisfies__lift_builtin_to_aosb
     {Σ : StaticModel}
     {V A B var : Type}
     {_varED : EqDecision var}
@@ -1026,14 +600,6 @@ Program Instance Satisfies__lift_builtin_to_aosb
     satisfies :=
         AppliedOperator'_symbol_A_satisfies_OpenTermB' V A B var;
 |}.
-Next Obligation.
-    intros.
-    unfold AppliedOperator'_symbol_A_satisfies_OpenTermB' in *.
-    eapply satisfies_ext.
-    { apply H. }
-    { assumption. }
-Qed.    
-Fail Next Obligation.
 
 #[export]
 Instance Satisfies__lift_builtin_to_aosbo
@@ -1074,7 +640,7 @@ Definition AppliedOperator'_symbol_builtin_satisfies_OpenTerm
 .
 
 #[export]
-Program Instance Satisfies__AppliedOperator'_symbol_builtin__OpenTerm
+Instance Satisfies__AppliedOperator'_symbol_builtin__OpenTerm
     {Σ : StaticModel}
     {V var : Type}
     {_varED : EqDecision var}
@@ -1093,19 +659,13 @@ Program Instance Satisfies__AppliedOperator'_symbol_builtin__OpenTerm
     satisfies :=
         AppliedOperator'_symbol_builtin_satisfies_OpenTerm ;
 |}.
-Next Obligation.
-    intros.
-    eapply satisfies_ext.
-    { apply H. }
-    { assumption. }
-Qed.
-Fail Next Obligation.
+
 
 #[local]
 Obligation Tactic := idtac.
 
 #[export]
-Program Instance Satisfies_builtin_expr
+Instance Satisfies_builtin_expr
     {Σ : StaticModel}:
     Satisfies
         Valuation
@@ -1117,16 +677,10 @@ Program Instance Satisfies_builtin_expr
         Expression_evaluate ρ e = Some (aoo_operand b)
     ) ;
 |}.
-Next Obligation.
-    intros. simpl in *.
-    erewrite Expression_evaluate_extensive_Some>[|apply H|].
-    { reflexivity. }
-    { assumption. }
-Qed.
-Fail Next Obligation.
+
 
 #[export]
-Program Instance Satisfies_asb_expr
+Instance Satisfies_asb_expr
     {Σ : StaticModel}:
     Satisfies
         Valuation
@@ -1138,30 +692,7 @@ Program Instance Satisfies_asb_expr
         Expression_evaluate ρ e = Some (aoo_app x)
     ) ;
 |}.
-Next Obligation.
-    intros. simpl in *.
-    erewrite Expression_evaluate_extensive_Some>[|apply H|].
-    { reflexivity. }
-    { assumption. }
-Qed.
-Fail Next Obligation.
 
-(*
-Definition GroundTerm_satisfies_RhsPattern
-    {Σ : StaticModel}
-    {V : Type}
-    `{Satisfies (V * builtin_value) Expression}
-    `{Satisfies (V * AppliedOperator' symbol builtin_value) Expression}
-    `{Satisfies (V * AppliedOperator' symbol builtin_value) (AppliedOperator' symbol Expression)}
-    :
-    (V*GroundTerm) -> RhsPattern -> Prop
-:= aoxyo_satisfies_aoxzo
-    V
-    symbol
-    builtin_value
-    Expression
-.
-*)
 
 #[export]
 Instance Satisfies__GroundTerm__RhsPattern
@@ -1184,7 +715,7 @@ Instance Satisfies__GroundTerm__RhsPattern
 Proof. apply _. Defined.
 
 #[export]
-Program Instance Satisfies_gt_var
+Instance Satisfies_gt_var
     {Σ : StaticModel}:
     Satisfies
         Valuation
@@ -1194,14 +725,6 @@ Program Instance Satisfies_gt_var
 := {|
     satisfies := (fun ρ g x => ρ !! x = Some g)
 |}.
-Next Obligation.
-    intros. simpl in *.
-    unfold Valuation in *.
-    eapply lookup_weaken.
-    { apply H0. }
-    { assumption. }
-Qed.
-Fail Next Obligation.
 
 #[export]
 Instance Subseteq_ValuationLR
@@ -1223,7 +746,7 @@ Instance VarsOf_ValuationLR
 
 
 #[export]
-Program Instance Satisfies_sym_bov
+Instance Satisfies_sym_bov
     {Σ : StaticModel}
     :
     Satisfies
@@ -1234,14 +757,10 @@ Program Instance Satisfies_sym_bov
 := {|
     satisfies := fun _ _ _ => False ;
 |}.
-Next Obligation.
-    simpl. auto with nocore.
-Qed.
-Fail Next Obligation.
 
 
 #[export]
-Program Instance Satisfies_Valuation_LR_SideCondition
+Instance Satisfies_Valuation_LR_SideCondition
     {Σ : StaticModel}
     :
     Satisfies
@@ -1254,14 +773,6 @@ Program Instance Satisfies_Valuation_LR_SideCondition
         satisfies ρ
         ;
 |}.
-Next Obligation.
-    simpl. intros.
-    inversion H; subst.
-    eapply satisfies_ext.
-    { apply H1. }
-    { assumption. }
-Qed.
-Fail Next Obligation.
 
 Definition GroundTerm_satisfies_OpenTerm
     {Σ : StaticModel}
@@ -1280,7 +791,7 @@ Instance Subseteq_unit {Σ : StaticModel}: SubsetEq unit :=
 .
 
 #[export]
-Program Instance Satisfies__GroundTerm__OpenTerm_inall
+Instance Satisfies__GroundTerm__OpenTerm_inall
     {Σ : StaticModel}
     :
     Satisfies
@@ -1291,26 +802,9 @@ Program Instance Satisfies__GroundTerm__OpenTerm_inall
 := {|
     satisfies := fun _ => GroundTerm_satisfies_OpenTerm ;
 |}.
-Next Obligation.
-    simpl. intros. assumption.
-Qed.
-Fail Next Obligation.
-
-
-(*
-#[export]
-Instance Satisfies_bv_ao'
-    {Σ : StaticModel}
-    :
-    Satisfies (Valuation * builtin_value) (AppliedOperator' symbol BuiltinOrVar)
-:= {|
-    satisfies := fun _ _ => False ;
-|}.
-*)
-
 
 #[export]
-Program Instance Satisfies_valuation_scs
+Instance Satisfies_valuation_scs
     {Σ : StaticModel}
     : Satisfies
         Valuation
@@ -1320,28 +814,9 @@ Program Instance Satisfies_valuation_scs
 := {|
     satisfies := fun ρ _ => Forall (satisfies ρ ());
 |}.
-Next Obligation.
-    intros. simpl in *.
-    rewrite Forall_forall. rewrite Forall_forall in H0.
-    intros x Hx. specialize (H0 x Hx).
-    eapply satisfies_ext.
-    { apply H. }
-    { assumption. }
-Qed.
-Fail Next Obligation.
 
-(*
 #[export]
-Instance Satisfies_bv_pureterm
-    {Σ : StaticModel}:
-    Satisfies (Valuation * builtin_value)
-    (AppliedOperator' symbol Expression)
-:= {|
-    satisfies := fun _ _ => False;
-|}.
-*)
-#[export]
-Program Instance
+Instance
     Satisfies_symbol_B
     {Σ : StaticModel}
     {V B var : Type}
@@ -1358,7 +833,3 @@ Program Instance
 := {|
     satisfies := fun _ _ _ => False ;
 |}.
-Next Obligation.
-    auto with nocore.
-Qed.
-
